Is0.lean
@@ -1,5 +1,4 @@
 import Is0.Basic
 import Is0.Is0
 import Is0.Lemmas
-import Is0.Original
 import Is0.Programs
