Is0/Programs.lean
@@ -1,3 +1,4 @@
+-- This file contains the MLIR program labeled `ORIGINAL` in the `nonzero-example` output.
 import Mathlib.Data.Nat.Prime
 import Mathlib.Data.Vector
 import Mathlib.Data.ZMod.Defs
@@ -8,19 +9,33 @@ import Is0.Basic
 
 namespace Risc0
 
--- The MLIR program labeled `ORIGINAL` in the `nonzero-example` output.
 open CirgenNotation in
-def is0OriginalProgram (x : Felt) (y : Felt) (z : Felt) : State × Option Prop :=
+def is0OriginalNondet (x : Felt) (y : Felt) (z : Felt) : State × Option (Felt × Felt) :=
   Cirgen.step { felts := Map.empty
               , props := Map.empty
               , buffers := Map.fromList [("in", [x]), ("out", [y, z])]
               , constraints := []
               } <|
-  "1"         ←ₐ 1;
   "x"         ←ₐ input[0];
   "isZeroBit" ←ₐ ??₀⟨"x"⟩;
   [0]         ←ₐ ⟨"isZeroBit"⟩;
   "invVal"    ←ₐ Inv ⟨"x"⟩;
+  [1]         ←ₐ ⟨"invVal"⟩;
+  "out[0]"    ←ₐ output[0];
+  ret ["out[0]", "out[1]"]
+
+open CirgenNotation in
+def is0OriginalConstraints (x : Felt) (isZeroBit : Felt) (invVal : Felt) : State × Option (Felt × Felt) :=
+  Cirgen.step { felts := Map.empty
+              , props := Map.empty
+              , buffers := Map.fromList [("in", [x]), ("out", [isZeroBit, invVal])]
+              , constraints := []
+              } <|
+  "1"         ←ₐ 1;
+  "x"         ←ₐ input[0];
+  "isZeroBit" ←ₐ isZeroBit;
+  [0]         ←ₐ ⟨"isZeroBit"⟩;
+  "invVal"    ←ₐ invVal;
   [1]         ←ₐ ⟨"invVal"⟩;
   "out[0]"    ←ₐ output[0];
   guard ⟨"out[0]"⟩ then
@@ -32,27 +47,5 @@ def is0OriginalProgram (x : Felt) (y : Felt) (z : Felt) : State × Option Prop :
     "x * out[1] - 1" ←ₐ ⟨"x * out[1]"⟩ - ⟨"1"⟩;
     ?₀ ⟨"x * out[1] - 1"⟩
   )
-
--- The MLIR program labeled `CONSTAINTS` in the `nonzero-example` output.
-open CirgenNotation in
-def is0ConstraintsProgram (x : Felt) (y : Felt) (z : Felt) : State × Option Prop :=
-  Cirgen.step { felts := Map.empty
-              , props := Map.empty
-              , buffers := Map.fromList [("in", [x]), ("out", [y, z])]
-              , constraints := []
-              } <| 
-  "1"                                   ←ₐ 1;
-  "true"                                ←ₐ ⊤;
-  "x"                                   ←ₐ input[0];
-  "isZeroBit"                           ←ₐ output[0];
-  "x = 0"                               ←ₐ ⟨"true"⟩ &₀ ⟨"x"⟩;
-  "IF isZeroBit THEN (x = 0) ELSE true" ←ₐ ⟨"true"⟩ guard ⟨"isZeroBit"⟩ & ⟨"x = 0"⟩;
-  "1 - isZeroBit"                       ←ₐ ⟨"1"⟩ - ⟨"isZeroBit"⟩;
-  "invVal"                              ←ₐ output[1];
-  "x * invVal"                          ←ₐ ⟨"x"⟩ * ⟨"invVal"⟩;
-  "x * invVal - 1"                      ←ₐ ⟨"x * invVal"⟩ - ⟨"1"⟩;
-  "x * invVal - 1 = 0"                  ←ₐ ⟨"true"⟩ &₀ ⟨"x * invVal - 1"⟩;
-  "result"                              ←ₐ ⟨"IF isZeroBit THEN (x = 0) ELSE true"⟩ guard ⟨"1 - isZeroBit"⟩ & ⟨"x * invVal - 1 = 0"⟩;
-  ret ["result"]
 
 end Risc0
